theories/unstructured.v
@@ -1,0 +1,440 @@
+
+
+
+
+Section Containment.
+  Variable P : regex -> regex -> dsl -> Prop.
+Reserved Notation "c0 <R= c1 ~> p" (at level 63).
+
+(*Tried as much as possible to stay within Henglein & Nielsen's formulation*)
+(*full_unf pf = ... ensures that pf <> pfix f. f
+  With an explicit fix rule, we would need to ensure guardedness*)
+Inductive c_ineq : regex -> regex -> dsl -> Prop :=
+| rule_shuffle c0 c1 c2 pf : full_unf pf = shuffle -> (c0 _+_ c1) _+_ c2 <R= c0 _+_ (c1 _+_ c2) ~> pf (*assoc  + *)
+
+
+| rule_shuffleinv c0 c1 c2 pf : full_unf pf = shuffleinv -> c0 _+_ (c1 _+_ c2)  <R= (c0 _+_ c1) _+_ c2 ~> pf (*assoc +*)
+
+| rule_retag c0 c1 pf: full_unf pf = retag -> c0 _+_ c1 <R= c1 _+_ c0 ~> pf (*comm +*)(*Other direction is redundant*)
+
+| rule_untagL c pf : full_unf pf = untagL -> Empt _+_ c <R= c ~> pf (* + neut r*)
+| rule_untagLinv c pf: full_unf pf = untagLinv -> c <R= Empt _+_ c ~> pf (*Possibly redundant*)
+
+| rule_untag c pf : full_unf pf = untag ->  c _+_ c <R= c ~> pf (*idem*)
+| rule_tagL c d pf : full_unf pf = tagL ->  c <R= c _+_ d ~> pf
+
+| rule_assoc c0 c1 c2 pf : full_unf pf = assoc ->  (c0 _;_ c1) _;_ c2 <R= c0 _;_ (c1 _;_ c2) ~> pf
+| rule_associnv c0 c1 c2 pf : full_unf pf = associnv -> c0 _;_ (c1 _;_ c2) <R=  (c0 _;_ c1) _;_ c2 ~> pf
+
+| rule_swap c pf : full_unf pf = swap -> (c _;_ Eps) <R= (Eps _;_ c) ~> pf (*New rule, from regex as types paper*)
+| rule_swapinv c pf : full_unf pf = swapinv -> (Eps _;_ c) <R= (c _;_ Eps) ~> pf
+
+| rule_proj c pf : full_unf pf = proj -> (Eps _;_ c) <R= c ~> pf
+| rule_projinv c pf : full_unf pf = projinv -> c <R=(Eps _;_ c) ~> pf
+
+| rule_abortR c pf : full_unf pf = abortR ->  c _;_ Empt <R= Empt ~> pf
+| rule_abortRinv c pf : full_unf pf = abortRinv ->  Empt  <R= c _;_ Empt ~> pf
+
+| rule_abortL c pf : full_unf pf = abortL -> Empt _;_ c <R=  Empt ~> pf
+| rule_abortLinv c pf : full_unf pf = abortLinv -> Empt  <R=  Empt _;_ c ~> pf
+
+| rule_distL c0 c1 c2 pf : full_unf pf = distL -> c0 _;_ (c1 _+_ c2) <R= (c0 _;_ c1) _+_ (c0 _;_ c2) ~> pf
+| rule_distLinv c0 c1 c2 pf : full_unf pf = distLinv -> (c0 _;_ c1) _+_ (c0 _;_ c2)  <R=  c0 _;_ (c1 _+_ c2) ~> pf
+
+| rule_distR c0 c1 c2 pf : full_unf pf = distR -> (c0 _+_ c1) _;_ c2 <R= (c0 _;_ c2) _+_ (c1 _;_ c2) ~> pf
+| rule_distRinv c0 c1 c2 pf : full_unf pf = distRinv ->  (c0 _;_ c2) _+_ (c1 _;_ c2)  <R= (c0 _+_ c1) _;_ c2 ~> pf
+
+
+| rule_wrap c pf : full_unf pf = wrap ->  Eps _+_ (c _;_ Star c) <R= Star c ~> pf
+| rule_wrapinv c pf : full_unf pf = wrapinv -> Star c  <R=Eps _+_ (c _;_ Star c) ~> pf
+
+| rule_drop c pf : full_unf pf = drop ->  Star (Eps _+_ c) <R= Star c ~> pf
+| rule_dropinv c pf : full_unf pf = dropinv ->  Star c <R= Star (Eps _+_ c) ~> pf (*Possibly redundant*)
+
+ (*We want to remove inner Eps, so we only keep this one for now*)
+(*Will the other direction be necessary?*)
+(*| ci_star_plus_inv c :  Star c  <R= Star (Eps _+_ c) (*Could possibly be removed but we are studying the computational interpretation of EQ rules*) *)
+
+| rule_cid c pf : full_unf pf = cid ->  c <R= c ~> pf
+
+(*| ci_sym c0 c1 (H: c0 =R=c1) : c1 =R=c0*)
+| rule_ctrans c0 c1 c2 pf p0 p1 : full_unf pf =  ctrans p0 p1 ->  c0 <R=c1 ~> p0 ->  c1 <R=c2 ~> p1 -> c0 <R=c2 ~> pf
+| rule_cplus c0 c0' c1 c1' pf p0 p1 : full_unf pf = cplus p0 p1 ->  c0 <R=c0' ~> p0 -> c1 <R=c1' ~> p1 -> c0 _+_ c1 <R=c0' _+_ c1' ~> pf
+| rule_cseq c0 c0' c1 c1' pf p0 p1 : full_unf pf = cseq p0 p1 ->  c0 <R=c0' ~> p0 -> c1 <R=c1' ~> p1 ->  c0 _;_ c1 <R=c0' _;_ c1' ~> pf
+| rule_cstar c0 c1 pf p : full_unf pf = cstar p ->  c0 <R=c1 ~> p -> Star c0 <R= Star c1 ~> pf  (*new context rule*) 
+(*| rule_cfix r r' (p  : dsl) : r <R= r' ~> p[d (cfix p) .: var_dsl] ->  r <R= r' ~> (cfix p) (*guarded p otherwise unsound*)*)
+| rule_guard a r r' pf p : full_unf pf = guard p -> P r r' p -> (Event a) _;_ r <R= (Event a) _;_ r' ~> pf
+ where "c1 <R= c2 ~> p" := (c_ineq c1 c2 p).
+End Containment.
+Hint Constructors c_ineq.
+Lemma c_ineq_gen_mon: monotone3 c_ineq. 
+Proof.
+unfold monotone3.
+intros. induction IN; eauto. 
+Qed.
+Hint Resolve c_ineq_gen_mon : paco.
+
+Notation "c0 < ( R ) = c1 ~> p" := (c_ineq R c0 c1 p)(at level 63).
+Definition INEQ c0 c1 p := paco3 c_ineq bot3 c0 c1 p.
+Notation "c0 <C= c1 ~> p" := (INEQ c0 c1 p)(at level 63).
+
+
+
+(*Ineffecient program*)
+Definition d6 := (ctrans (cstar wrapinv)
+              (ctrans drop
+                 (ctrans wrapinv
+                    (ctrans
+                       (cplus cid
+                          (ctrans assoc
+                             (cseq cid
+                                (cfix
+                                   (ctrans (cseq cid dropinv)
+                                      (ctrans (cseq cid (cstar wrap))
+                                         (cfix
+                                            (ctrans (cseq wrapinv cid)
+                                               (ctrans distR (ctrans (cplus proj cid) (ctrans (ctrans ((ctrans
+             (ctrans
+                (ctrans
+                   (ctrans
+                      (ctrans
+                         (cplus
+                            (ctrans (cstar wrapinv)
+                               (ctrans drop (ctrans wrapinv (ctrans (cplus cid (ctrans assoc (guard ((var_dsl 1))))) wrap))))
+                            (ctrans assoc (guard ((var_dsl 0))))) tagL) retag) (cplus cid (cplus projinv cid)))
+                (cplus cid distRinv)) (cplus cid (cseq cid dropinv)))) wrap) drop)))))))))))
+                       wrap)))).
+
+
+(*Uses two fixpoints*)
+Lemma star_star_co_ineq : forall a,  (Star (Star (Event a))) <C= (Star (Event a)) ~> d6.
+Proof.
+move=> a.  pfold.
+
+apply: rule_ctrans=>//. apply: rule_cstar=>//. apply: rule_wrapinv=>//.
+
+apply/rule_ctrans=>//. apply/rule_drop=>//.
+apply/rule_ctrans=>//. apply/rule_wrapinv=>//.
+apply/rule_ctrans=>//. 2: { apply/rule_wrap=>//. }
+apply/rule_cplus=>//. apply/rule_cid=>//.
+apply/rule_ctrans=>//. apply/rule_assoc=>//.
+(*apply/rule_guard=>//. left. pcofix CIH. pfold*)  
+apply/rule_cseq=>//. apply/rule_cid=>//. (*Don't use rule_guard yet*) (*apply/rule_guard=>//. left=>//. pfold.*)
+
+pfold_reverse. pcofix CIH. pfold. (*pcofix before cfix*)
+(*apply/rule_cfix=>//. simpl=>//. *)
+
+apply: rule_ctrans. rewrite /full_unf //=. 
+apply/rule_cseq=>//. apply/rule_cid=>//. apply/rule_dropinv=>//.
+
+apply/rule_ctrans=>//. apply/rule_cseq=>//. apply/rule_cid=>//. apply/rule_cstar/rule_wrap=>//. 
+
+
+pfold_reverse=>//. pcofix CIH2=>//. pfold=>//. (*pcofix before cfix*)
+(*apply/rule_cfix=>//. simpl=>//. *)
+
+
+
+apply/rule_ctrans. rewrite /full_unf //=. apply/rule_cseq=>//. apply/rule_wrapinv=>//. apply/rule_cid=>//.
+apply/rule_ctrans=>//. apply/rule_distR=>//.
+apply/rule_ctrans=>//. apply/rule_cplus=>//. apply/rule_proj=>//. apply/rule_cid=>//.
+apply/rule_ctrans=>//. 2: { apply/rule_drop=>//. }
+apply/rule_ctrans=>//. 2: { apply/rule_wrap=>//. }
+
+(*Unset Printing Notations.*)
+apply/rule_ctrans=>//. 2: { apply/rule_cplus=>//. apply/rule_cid=>//. apply/rule_cseq=>//. apply/rule_cid=>//. apply/rule_dropinv=>//. }
+apply/rule_ctrans=>//. 2: { apply/rule_cplus=>//. apply/rule_cid=>//. apply/rule_distRinv=>//. }
+
+
+
+
+apply/rule_ctrans=>//. 2: { apply/rule_cplus=>//. apply/rule_cid=>//. apply/rule_cplus=>//. apply/rule_projinv=>//. apply/rule_cid=>//. }
+apply/rule_ctrans=>//. 2: { apply/rule_retag=>//. }
+apply/rule_ctrans=>//. 2: { apply/rule_tagL=>//. }
+
+
+apply/rule_cplus=>//. 
+
+apply/rule_ctrans=>//. apply/rule_cstar/rule_wrapinv=>//. 
+apply/rule_ctrans=>//. apply/rule_drop=>//.
+apply/rule_ctrans=>//. apply/rule_wrapinv=>//.
+apply/rule_ctrans=>//. 2: { apply/rule_wrap=>//. }
+apply/rule_cplus=>//. apply/rule_cid=>//.
+apply/rule_ctrans=>//. apply/rule_assoc=>//.
+apply/rule_guard=>//. right. apply/CIH.
+
+apply/rule_ctrans=>//. apply/rule_assoc=>//.
+apply/rule_guard=>//. right.  apply/CIH2.
+Qed.
+
+
+
+
+
+
+
+
+
+
+
+(*
+Definition ex_eq {A : eqType} (l: seq A) (F0 F1 : A -> regex) R  := forall a, a \in l -> R (F0 a) (F1 a).
+
+Lemma eq_big_plus2 : forall (l : seq A) F1 F2 R, ex_eq l F1 F2 (c_eq R) ->
+   \big[Plus/Empt]_(i <- l) F1 i = ⟨R⟩ = \big[Plus/Empt]_(i <- l) F2 i.
+Proof.
+move=> + F1 F2 R. 
+rewrite /ex_eq. elim=>//.
+move=> _. rewrite !big_nil//.
+move=> a l IH Hin. rewrite !big_cons. rewrite Hin //. 
+eq_m_left2.
+Qed.
+
+(*Necessary to use ssreflect under for rewriting*)
+Add Parametric Morphism R : (Under_rel regex (c_eq R)) with
+signature (c_eq R ==> c_eq R ==> flip impl) as under_c_eq. 
+Proof.
+move=> x y HC x0 y0 HC'. intro. move: H. rewrite UnderE. move=> HC''. apply/c2_trans.  eauto. apply/c2_trans. eauto. apply/c2_sym. eauto.
+Qed.
+
+Add Parametric Morphism R : (Under_rel regex (c_eq R)) with
+signature (c_eq R ==> c_eq R ==> impl) as under_c_eqc3. 
+Proof.
+move=> x y HC x0 y0 HC'. intro. move: H. rewrite UnderE. move=> HC''.  apply/c2_trans;last by eauto. apply/c2_trans;last by eauto. apply/c2_sym. eauto.
+Qed.
+
+(*This has to be proved by induction because I cannot use ssreflects big_split since commutativity is over c_eqc, and not leibniz equality*)
+Lemma split_plus2 : forall R (B: eqType) l (P P' : B -> regex),
+\big[Plus/Empt]_(a <- l) (P a _+_ P' a) = ⟨R⟩ = \big[Plus/Empt]_(a <- l) (P a) _+_ \big[Plus/Empt]_(a <- l) (P' a).  
+Proof.
+move => R B + P P'.
+elim=>//. rewrite !big_nil // eqs2 //.
+move=> a l IH. rewrite !big_cons. eq_m_left2. rewrite IH. eauto.
+Qed.
+
+Lemma factor_seq_l2 : forall R (B: eqType) l (P: B -> regex) c,
+\big[Plus/Empt]_(a <- l) (c _;_ P a) =⟨R⟩=  c _;_ (\big[Plus/Empt]_(a <- l) (P a)).
+Proof.
+move=> R B +P c. elim=>//=. rewrite !big_nil eqs2 //.
+move=> a l IH. rewrite !big_cons eqs2 //= IH //.
+Qed.
+
+
+
+Lemma factor_seq_r2 : forall R (B: eqType) l (P: B -> regex) c,
+\big[Plus/Empt]_(a <- l) (P a _;_ c) =⟨R⟩= (\big[Plus/Empt]_(a <- l) (P a)) _;_ c.
+Proof.
+move=> R B +P c. elim=>//=. rewrite !big_nil eqs2 //.
+move=> a l IH. rewrite !big_cons eqs2 //= IH //.
+Qed.
+
+
+Lemma big_event_notin2 R : forall l a, a \notin l -> \big[Plus/Empt]_(i <- l) ((Event i)_;_(i \ Event a)) =⟨R⟩= Empt. 
+Proof.
+elim=>//=. move=> a _. rewrite !big_nil //.
+move=> a l IH a0 /=. rewrite !inE. move/andP=>[] Hneq Hin.
+rewrite !big_cons. rewrite (negbTE Hneq) IH // !eqs2 //.
+Qed.
+
+Lemma big_event_in2 R : forall l a, a \in l -> \big[Plus/Empt]_(i <- l) ((Event i)_;_(i \ Event a)) =⟨R⟩= Event a. 
+Proof.
+elim=>//=.
+move=> a l IH a0 /=.
+rewrite !inE. move/orP. case. move/eqP=>Heq;subst.
+rewrite big_cons eqxx //= !eqs2.
+case Hcase: (a \in l). rewrite IH. apply/c2_plus_idemp=>//. rewrite Hcase//.
+rewrite big_event_notin2 //. rewrite Hcase//.
+move=>Hin. rewrite big_cons IH //.
+case: (eqVneq a a0). move=>Heq;subst. rewrite !eqs2 //.
+move=>Hneq. rewrite !eqs2 //=.
+Qed.
+
+(*Shorten this proof*)
+Lemma derive_seq2 : forall R a r r', a \ (r _;_ r') =⟨R⟩= ((a \ r) _;_ r') _+_ (o (r) _;_ a \ r').
+Proof.
+move=> R a r r' /=. case Hcase: (nu r)=>/=. rewrite /o Hcase /= eqs2 //.
+rewrite /o Hcase !eqs2 //.
+Qed.
+
+
+
+(*Why we need star ctx, 
+  Proof below is by induction on regex syntax, to use IH, we need c0 = c1 -> c0* = c1*
+  This cannot be derived, as we need some coinductive rule, namely c_fix, which requires
+  us to show this decomposition rule to be useful
+*)
+
+
+(*Uses c_star_plus!*)
+Lemma star_o2 : forall R c c', Star ((o c) _+_ c') =⟨R⟩ = Star c'.
+Proof. 
+move=> R c c'. 
+rewrite /o. case Hcase: (nu c);last by rewrite eqs2 //. clear Hcase.
+rewrite c2_star_plus //.
+Qed.
+
+Lemma derive_unfold2 : forall R c, c =⟨R⟩= o c _+_ \big[Plus/Empt]_(a : A) (Event a _;_ a \ c). 
+Proof.
+move=>R. 
+elim.
+- rewrite /o /=. under eq_big_plus2. move=> a Hin. rewrite !eqs2. over. rewrite plus_empt2 eqs2 //.
+- rewrite /o /=. under eq_big_plus2. move=> a Hin. rewrite !eqs2. over. rewrite plus_empt2 eqs2 //.
+- move => s. rewrite big_event_in2 /o //= ?eqs2 // mem_index_enum //. 
+- move=> r HQ r' HQ'. rewrite o_plus2 /=. 
+  under eq_big_plus2. move=> a Hin. rewrite eqs2. over. 
+  rewrite split_plus2. 
+  apply/c2_trans. apply/c2_plus_ctx. apply: HQ. apply: HQ'. eq_m_left2.  
+  rewrite c2_plus_comm. eq_m_left2.
+- move=> r HQ r' HQ'. 
+  under eq_big_plus2. move=> a Hin. 
+  rewrite derive_seq2 !eqs2 -!c2_seq_assoc seq_comm_o2 (c2_seq_assoc _ (o r)).
+  over.
+  rewrite split_plus2 !factor_seq_l2 !factor_seq_r2  o_seq2. 
+  apply/c2_trans. apply/c2_seq_ctx. apply: HQ. apply: HQ'.
+  apply/c2_trans. 2 : {  apply/c2_plus_ctx. apply/c2_refl. apply/c2_plus_ctx. apply/c2_seq_ctx. apply/c2_refl.
+                        apply/c2_sym. apply: HQ'. apply/c2_refl. }
+  rewrite !eqs2. eq_m_left2. 
+- move=> r HQ /=. 
+  under eq_big_plus2. move=> a Hin. rewrite -c2_seq_assoc. rewrite {2}HQ. over.
+  rewrite factor_seq_r2. rewrite {1}HQ.
+  rewrite {1}star_o2.
+  rewrite {1}star_o2. 
+  rewrite c2_unfold. done.
+ (*We need c_star_plus here*)
+Qed.
+*)
+
+
+
+
+
+
+Lemma star_star_ind_eq : forall c, Star c =⟨nil⟩= Star (Star c).
+Proof. 
+intros. (* (Star c, (Star (Star c))) in pgfp(bot2)(F)*) 
+ (* (Star c, (Star (Star c))) in F(bot2 union R*) 
+apply:c_trans. apply:derive_unfold. apply:c_trans.
+2: { apply:c_sym. apply:derive_unfold. } 
+apply:c_plus_ctx. done. 
+move: (index_enum A) => l. 
+elim: l. rewrite !big_nil. done. 
+intros. rewrite !big_cons. apply:c_plus_ctx;last done.  (*bot2 union gfp(F)*)
+clear H. simpl. 
+apply:c_seq_ctx. done. rewrite c_seq_assoc. apply:c_seq_ctx. done.
+
+pfold_reverse.
+move: c. pcofix C_useless.
+intro. pfold.
+(*
+left. (*move: a c. pcofix CIH. intros.*)
+
+(*2: {  done. }
+sum_reshape. 
+apply c_co_sum. intros.
+simp_premise.*)
+
+pfold. simpl.*)
+(* rewrite c_seq_assoc. apply c_seq_ctx. done. *)
+apply:c_trans. apply:derive_unfold. apply:c_trans.
+2: { apply:c_sym. apply:derive_unfold. } 
+apply:c_plus_ctx. done. 
+move: (index_enum A) => l'. 
+elim: l'. rewrite !big_nil. done. 
+intros. rewrite !big_cons. apply:c_plus_ctx;last done.  
+clear H. 
+apply:c_fix. left. 
+(* apply:c_seq_ctx. done. pfold_reverse. *) 
+(*(a0 \ Star c, 
+   a0 \ (Star c _;_ (Star (Star c)))*)
+move: a0.  (*(r0,r1) \in pgfp(bot2)(F)
+            (forall (a0 : event) (c : regex), 
+            (a0 \ Star c, a0 \ (Star c ; (Star (Star c))) \in R)
+            R subset F(R)
+               (r0,r1) \in pgfp(R)(F)
+
+*)
+pcofix CIH. intros. pfold.
+simpl. rewrite c_plus_idemp.
+(* apply:c_fix.  
+
+left. move: a0 c. pcofix CIH. intros.*)
+
+(*pfold. simpl.*)
+(*apply/CIH.
+
+unfold_tac.
+sum_reshape. 
+apply c_co_sum. intros.
+simp_premise.
+left.*)
+
+
+(*generalize x0. pcofix CIH2. intros.*) (*Coinduction principle*)
+(*pfold. *)
+(*rewrite c_plus_idemp. *)
+rewrite c_seq_assoc. 
+ apply c_seq_ctx. done.
+apply:c_trans. apply:derive_unfold. apply:c_trans.
+2: { apply:c_sym. apply:derive_unfold. } 
+apply:c_plus_ctx. done. 
+move: (index_enum A) => l'. 
+elim: l'. rewrite !big_nil. done. 
+intros. rewrite !big_cons. apply:c_plus_ctx;last done.  
+clear H. apply:c_fix. right.
+apply: CIH.
+
+(*ones := cons 1 ones*)
+Qed. 
+*)
+
+
+
+
+
+
+
+
+
+
+
+
+
+
+Inductive contains_gen bisim : regex -> regex -> Prop :=
+ contains_con c0 c1 (H0: forall e, bisim (e \ c0) (e \ c1) : Prop ) (H1: nu c0 -> nu c1) : contains_gen bisim c0 c1.
+Lemma contains_gen_mon: monotone2 contains_gen. 
+Proof.
+unfold monotone2. intros.  constructor. inversion IN. intros.
+auto. inversion IN. auto.  
+Qed.
+Hint Resolve contains_gen_mon : paco.
+
+
+
+Definition Contains c0 c1 := paco2 contains_gen bot2 c0 c1.
+Hint Unfold  Contains : core.
+
+Lemma Contains_der : forall c0 c1, Contains c0 c1 -> forall e,  Contains (e \ c0) (e \ c1).
+Proof.
+intros. punfold H.  inv H. move: (H0 e). case. done. done.
+Qed.
+
+Lemma Contains_nu : forall c0 c1, Contains c0 c1 ->  nu ( c0) -> nu ( c1).
+Proof.
+intros. punfold H.  inv H. eauto. 
+Qed.
+
+(*Definition bisim_proj R r0 r1 (H: bisimilarity_gen R r0 r1) :=
+match H with 
+| bisimilarity_con _ _ H0 H1 => H0
+end.
+*)
+
+Definition contains (r0 r1 : regex) := forall s, Match s r0 -> Match s r1.
+
+Theorem containsP : forall c0 c1, contains c0 c1 -> Contains c0 c1.
+Proof.
+pcofix CIH. intros. pfold. constructor.
+- intros. right. apply CIH.  move=> s.  rewrite -!deriveP. eauto.
+  move: (H0 nil). rewrite !matchbP /matchb //=. 
+Qed.
